Setoid moment

theories/GraphCore/GraphRewriting.v
@@ -1,5 +1,5 @@
 From stdpp Require Export pmap gmap decidable.
-Require Import TensorGraph.
+Require Import TensorGraph TensorGraphSemantics TensorGraphFacts.
 Require Import HyperGraph.
 Require Import TESyntax.
 Require Import Aux_pos.
@@ -10,381 +10,6 @@ Local Open Scope nat_scope.
 Section DPO.
 
   Context {T : Type}.
-
-  Definition all_vertices (H : HyperGraph T) : Pset :=
-    map_fold (fun k h s => (list_to_set h.1.2 ∪ list_to_set h.2) ∪ s)
-    (H.(hypervertices)) (H.(hyperedges)).
-
-
-  Definition compose_graphs_aux {n m o} (tgl : CospanHyperGraph T n m) (tgr : CospanHyperGraph T m o) : CospanHyperGraph T n o :=
-    let connected_substs := propogate_subst (vzip (tgl.(outputs)) (tgr.(inputs))) in
-    relabel_graph (subst_by_vec connected_substs)
-      (tgl.(inputs) ->
-        hg_add_vertices (tgl.(hedges) ∪ tgr.(hedges)) (list_to_set tgr.(inputs) ∖ (vertices_hg tgl ∪ vertices_hg tgr))
-          <- tgr.(outputs)).
-
-  (* Reserved Notation "tgl ; tgr" (at level 50). *)
-  Definition compose_graphs {n m o} (tgl : CospanHyperGraph T n m) (tgr : CospanHyperGraph T m o) : CospanHyperGraph T n o :=
-    let connected_substs :=
-        propogate_subst (vzip (vmap (bcons false) tgl.(outputs)) (vmap (bcons true) tgr.(inputs))) in
-     relabel_graph (subst_by_vec connected_substs) ((vmap (bcons false) tgl.(inputs)) ->
-      hg_add_vertices (tgl.(hedges) ⊎ tgr.(hedges))
-        ((list_to_set (vmap (bcons true) tgr.(inputs)) ∖
-          (vertices_hg (reindex_graph (bcons false) (relabel_graph (bcons false) tgl)) ∪
-           vertices_hg (reindex_graph (bcons true) (relabel_graph (bcons true) tgr)))))
-           <- (vmap (bcons true) tgr.(outputs))).
-
-
-  Definition compose_graphs_unsafe {n m o} (tgl : CospanHyperGraph T n m) (tgr : CospanHyperGraph T m o) : CospanHyperGraph T n o :=
-    tgl.(inputs) ->  hg_add_vertices (tgl.(hedges) ∪ tgr.(hedges)) (list_to_set (tgr.(inputs)) ∖ (vertices_hg tgl ∪ vertices_hg tgr)) <- tgr.(outputs).
-
-Lemma compose_graphs_to_compose_graphs_aux {n m o}
-  (tgl : CospanHyperGraph T n m) (tgr : CospanHyperGraph T m o) :
-  compose_graphs tgl tgr = compose_graphs_aux
-    (reindex_graph (bcons false) (relabel_graph (bcons false) tgl))
-    (reindex_graph (bcons true) (relabel_graph (bcons true) tgr)).
-Proof.
-  reflexivity.
-Qed.
-
-Lemma compose_graphs_aux_to_compose_graphs_unsafe {n m o} (tgl : CospanHyperGraph T n m) (tgr : CospanHyperGraph T m o) :
-  tgl.(outputs) = tgr.(inputs) ->
-  compose_graphs_aux tgl tgr = compose_graphs_unsafe tgl tgr.
-Proof.
-  intros.
-  unfold compose_graphs_aux.
-  rewrite H.
-  unfold relabel_graph.
-  rewrite Vector.map_ext with (g:=(λ x : _, x)) by apply subst_by_vec_id.
-  rewrite Vector.map_id.
-  simpl.
-  rewrite Vector.map_ext with (g:=(λ x : _, x)) by apply subst_by_vec_id.
-  rewrite Vector.map_id.
-  simpl.
-  rewrite relabel_hg_id' by apply subst_by_vec_id.
-  reflexivity.
-Qed.
-
-
-
-
-Lemma inputs_add_top_loops {n m m'}
-  (tg : CospanHyperGraph T (n + m) (n + m')) :
-  (add_top_loops tg).(inputs) =
-  vmap (subst_by_vec (propogate_subst
-    (vzip (vsplitl tg.(outputs))
-      (vsplitl tg.(inputs)))))
-      (vsplitr tg.(inputs)).
-Proof.
-  induction n; [cbn; now rewrite Vector.map_id|].
-  cbn [add_top_loops].
-  rewrite IHn.
-  destruct tg as [hg ins outs].
-  induction ins as [insl insr] using vec_add_inv.
-  induction outs as [outsl outsr] using vec_add_inv.
-  induction insl as [i insl] using vec_S_inv.
-  induction outsl as [o outsl] using vec_S_inv.
-  cbn -[Vector.append].
-  rewrite 2 vsplitl_app, vsplitr_app.
-  cbn.
-  rewrite 2 vsplitl_map, 2 vsplitl_app.
-  rewrite vsplitr_map, vsplitr_app.
-  rewrite Vector.map_map.
-  apply Vector.map_ext.
-  intros p.
-  apply susbt_by_vec_propogate_helper.
-Qed.
-
-
-Lemma outputs_add_top_loops {n m m'}
-  (tg : CospanHyperGraph T (n + m) (n + m')) :
-  (add_top_loops tg).(outputs) =
-  vmap (subst_by_vec (propogate_subst
-    (vzip (vsplitl tg.(outputs))
-      (vsplitl tg.(inputs)))))
-      (vsplitr tg.(outputs)).
-Proof.
-  induction n; [cbn; now rewrite Vector.map_id|].
-  cbn [add_top_loops].
-  rewrite IHn.
-  destruct tg as [hg ins outs].
-  (* cbn in ins, outs. *)
-  induction ins as [insl insr] using vec_add_inv.
-  induction outs as [outsl outsr] using vec_add_inv.
-  induction insl as [i insl] using vec_S_inv.
-  induction outsl as [o outsl] using vec_S_inv.
-  cbn -[Vector.append].
-  rewrite 2 vsplitl_app, vsplitr_app.
-  cbn.
-  rewrite 2 vsplitl_map, 2 vsplitl_app.
-  rewrite vsplitr_map, vsplitr_app.
-  rewrite Vector.map_map.
-  apply Vector.map_ext.
-  intros p.
-  apply susbt_by_vec_propogate_helper.
-Qed.
-
-
-Lemma hedges_add_top_loops {n m m'}
-  (tg : CospanHyperGraph T (n + m) (n + m')) :
-  (add_top_loops tg).(hedges) =
-  relabel_hg (subst_by_vec (propogate_subst
-    (vzip (vsplitl tg.(outputs))
-      (vsplitl tg.(inputs)))))
-      (hg_add_vertices tg.(hedges)
-      (list_to_set (vsplitl tg.(inputs)))).
-Proof.
-  induction n; [cbn; now rewrite relabel_hg_id, hg_add_vertices_empty|].
-  cbn [add_top_loops].
-  rewrite IHn.
-  destruct tg as [hg ins outs].
-  (* cbn in ins, outs. *)
-  induction ins as [insl insr] using vec_add_inv.
-  induction outs as [outsl outsr] using vec_add_inv.
-  induction insl as [i insl] using vec_S_inv.
-  induction outsl as [o outsl] using vec_S_inv.
-  cbn -[Vector.append union].
-  rewrite 2 vsplitl_app.
-  cbn -[union].
-  rewrite 2 vsplitl_map, 2 vsplitl_app.
-  rewrite 4 relabel_hg_add_vertices, hg_add_vertices_union.
-  f_equal.
-  - rewrite relabel_hg_compose.
-    apply relabel_hg_ext.
-    intros p; cbn.
-    now rewrite susbt_by_vec_propogate_helper.
-  - rewrite <- set_map_union_L.
-    rewrite vec_to_list_map, <- (set_map_list_to_set_L (SA:=Pset)).
-    rewrite <- set_map_union_L.
-    rewrite set_map_compose_L.
-    apply set_map_ext_L.
-    intros ? _.
-    cbn.
-    apply susbt_by_vec_propogate_helper.
-Qed.
-
-Lemma add_top_loops_alt {n m m'}
-  (tg : CospanHyperGraph T (n + m) (n + m')) :
-  add_top_loops tg =
-  relabel_graph (subst_by_vec (propogate_subst
-    (vzip (vsplitl tg.(outputs))
-      (vsplitl tg.(inputs)))))
-    (vsplitr tg.(inputs) ->
-      hg_add_vertices tg.(hedges) (list_to_set (vsplitl tg.(inputs)))
-      <- vsplitr tg.(outputs)).
-Proof.
-  apply cohg_ext.
-  - apply hedges_add_top_loops.
-  - apply inputs_add_top_loops.
-  - apply outputs_add_top_loops.
-Qed.
-
-
-
-Lemma add_top_loop'_correct {n m}
-  (tg : CospanHyperGraph T (S n) (S m)) :
-  add_top_loop' tg ≡ᵥ add_top_loop tg.
-Proof.
-  apply cohg_ext'; [done..|].
-  cbn.
-  unfold add_top_loop', add_top_loop.
-  unfold isolated_vertices.
-  rewrite 2 referrenced_vertices_relabel_graph.
-  cbn -[union difference].
-  change (referrenced_vertices _) with
-    (referrenced_vertices (vtl (inputs tg) -> hg_add_vertices tg {[vhd (inputs tg)]} <-
-        vtl (outputs tg))).
-  apply leibniz_equiv_iff, set_subseteq_antisymm. 1:{
-    apply difference_mono; [|done].
-    f_equiv.
-    apply union_mono_r.
-    set_solver.
-  }
-  apply (subseteq_union_r _ _ _).1.
-  rewrite (union_comm _ (_ ∖ _)), difference_union.
-  rewrite <- set_map_union.
-  f_equiv.
-  apply union_subseteq, conj, union_subseteq_l', union_subseteq_r.
-  apply singleton_subseteq_l.
-  rewrite (difference_singleton_l_case_L (vhd (inputs tg)) (vertices_hg tg)).
-  case_decide as Hivert.
-  - unfold vertices_hg in Hivert.
-    set_solver.
-  - apply elem_of_union_l, elem_of_union_l, elem_of_singleton.
-    done.
-Qed.
-
-
-Lemma isolated_vertices_add_top_loop {n m} (cohg : CospanHyperGraph T (S n) (S m)) :
-  isolated_vertices (add_top_loop cohg) =
-  isolated_vertices cohg ∪ ({[(vhd (inputs cohg))]} ∖ referrenced_vertices (add_top_loop cohg)).
-Proof.
-  unfold isolated_vertices, add_top_loop.
-  rewrite referrenced_vertices_relabel_graph.
-  cbn -[difference union].
-  unfold_leibniz.
-  apply set_subseteq_antisymm.
-  - intros fk [(k & -> & Hkih)%elem_of_map Hkr]%elem_of_difference.
-    rewrite union_comm_L in Hkih.
-    rewrite <- difference_union in Hkih.
-    rewrite elem_of_union, elem_of_difference, elem_of_singleton in Hkih.
-    destruct Hkih as [[Hkh Hkni] | ->].
-    + rewrite fn_lookup_singleton_case in *.
-      case_decide as Hok.
-      * subst k.
-        apply elem_of_union_r, elem_of_difference.
-        split; [|done].
-        now apply elem_of_singleton.
-      * apply elem_of_union_l.
-        apply elem_of_difference, (conj Hkh).
-        intros Hk.
-        apply Hkr.
-        apply elem_of_map.
-        exists k.
-        split; [now rewrite fn_lookup_singleton_ne|].
-        clear Hkh Hkr.
-        unfold referrenced_vertices in Hk.
-        rewrite (Vector.eta (inputs cohg)), (Vector.eta (outputs cohg)) in Hk.
-        cbn -[union] in *.
-        set_solver.
-    + rewrite fn_lookup_singleton_r in *.
-      apply elem_of_union_r, elem_of_difference.
-      split; [|done].
-      now apply elem_of_singleton.
-  - apply union_subseteq, conj.
-    + intros k [Hkh Hkr]%elem_of_difference.
-      unfold referrenced_vertices in Hkr.
-      rewrite (Vector.eta (inputs cohg)), (Vector.eta (outputs cohg)) in Hkr.
-      cbn -[union] in *.
-      apply elem_of_difference, conj.
-      * apply elem_of_map.
-        exists k.
-        rewrite fn_lookup_singleton_ne by set_solver + Hkr.
-        split; [done|].
-        now apply elem_of_union_r.
-      * intros (k' & -> & Hk')%elem_of_map.
-        rewrite fn_lookup_singleton_case in *.
-        case_decide as Hok'; [set_solver + Hkr|].
-        apply Hkr.
-        set_solver +Hk'.
-    + rewrite <- subseteq_union_r.
-      rewrite union_comm_L, difference_union.
-      apply singleton_subseteq_l, elem_of_union_l.
-      apply elem_of_map.
-      exists (vhd (inputs cohg)).
-      rewrite fn_lookup_singleton_r.
-      split; [done|].
-      now apply elem_of_union_l, elem_of_singleton.
-Qed.
-
-
-
-Lemma norm_verts_add_top_loop {n m} (cohg : CospanHyperGraph T (S n) (S m)) :
-  norm_verts (add_top_loop cohg) = norm_verts (add_top_loop (norm_verts cohg)).
-Proof.
-  apply cohg_ext'; [done..|].
-  cbn.
-  rewrite 2 isolated_vertices_add_top_loop.
-  rewrite isolated_vertices_norm_verts.
-  done.
-Qed.
-
-Lemma norm_verts_add_top_loops {n m o} (cohg : CospanHyperGraph T (n + m) (n + o)) :
-  norm_verts (add_top_loops cohg) = norm_verts (add_top_loops (norm_verts cohg)).
-Proof.
-  induction n; [cbn; now rewrite norm_verts_idemp|].
-  cbn.
-  now rewrite IHn, norm_verts_add_top_loop, <- IHn.
-Qed.
-
-#[export] Instance add_top_loop_proper {n m} :
-  Proper (@cohg_vert_eq T (S n) (S m) ==> cohg_vert_eq) add_top_loop.
-Proof.
-  intros cohg cohg' Heq.
-  hnf.
-  rewrite norm_verts_add_top_loop, Heq, <- norm_verts_add_top_loop.
-  done.
-Qed.
-
-#[export] Instance add_top_loop'_proper {n m} :
-  Proper (@cohg_vert_eq T (S n) (S m) ==> cohg_vert_eq) add_top_loop'.
-Proof.
-  intros cohg cohg' Heq.
-  rewrite 2 add_top_loop'_correct.
-  now f_equiv.
-Qed.
-
-#[export] Instance add_top_loops_proper {n m o} :
-  Proper (@cohg_vert_eq T (n + m) (n + o) ==> cohg_vert_eq) add_top_loops.
-Proof.
-  intros cohg cohg' Heq.
-  hnf.
-  rewrite norm_verts_add_top_loops, Heq, <- norm_verts_add_top_loops.
-  done.
-Qed.
-
-Lemma add_top_loops'_correct {n m o}
-  (tg : CospanHyperGraph T (n + m) (n + o)) :
-  add_top_loops' tg ≡ᵥ add_top_loops tg.
-Proof.
-  induction n; [done|].
-  cbn.
-  rewrite IHn.
-  now rewrite add_top_loop'_correct.
-Qed.
-
-
-Lemma add_top_loops_alt_vert_eq {n m m'}
-  (tg : CospanHyperGraph T (n + m) (n + m')) :
-  add_top_loops tg ≡ᵥ
-  relabel_graph (subst_by_vec (propogate_subst
-    (vzip (vsplitl tg.(outputs))
-      (vsplitl tg.(inputs)))))
-    (vsplitr tg.(inputs) ->
-      hg_add_vertices tg.(hedges)
-      (list_to_set (vsplitl tg.(inputs)) ∖ vertices_hg tg)
-      <- vsplitr tg.(outputs)).
-Proof.
-  rewrite add_top_loops_alt.
-  apply relabel_graph_cohg_vert_eq.
-  apply cohg_ext'; [done..|].
-  cbn.
-  unfold isolated_vertices.
-  cbn.
-  rewrite 2 referrenced_vertices_decomp.
-  cbn.
-  rewrite vertices_hg_decomp.
-  rewrite <- 3 difference_difference_l_L, difference_union_L.
-  set_solver.
-Qed.
-
-
-
-Lemma compose_graphs_alt_aux_correct {n m o}
-  (tgl : CospanHyperGraph T n m) (tgr : CospanHyperGraph T m o) :
-  hyperedges tgl ##ₘ hyperedges tgr ->
-  add_top_loops (swapped_stack_graphs_aux tgl tgr) ≡ᵥ
-    compose_graphs_aux tgl tgr.
-Proof.
-  intros Hdisj.
-  rewrite add_top_loops_alt_vert_eq.
-  cbn.
-  rewrite 2 vsplitl_app, 2 vsplitr_app.
-  unfold compose_graphs_aux.
-  rewrite vertices_hg_union by done.
-  reflexivity.
-Qed.
-
-Lemma compose_graphs_alt_correct {n m o}
-  (tgl : CospanHyperGraph T n m) (tgr : CospanHyperGraph T m o) :
-  add_top_loops (swapped_stack_graphs tgl tgr) ≡ᵥ
-    compose_graphs tgl tgr.
-Proof.
-  rewrite compose_graphs_to_compose_graphs_aux.
-  rewrite <- compose_graphs_alt_aux_correct; [rewrite 2 reindex_relabel_graph; done|].
-  cbn.
-  now apply (kmap_inj2_disjoint _).
-Qed.
 
 Lemma relabel_stack_graphs_aux {n m n' m'} (cohg : CospanHyperGraph T n m)
   (cohg' : CospanHyperGraph T n' m') f :
@@ -1910,7 +1535,7 @@ Definition decompose_left {n m} (G : CospanHyperGraph T n m) (L : HyperGraph T) 
   H.(inputs) -> {| hyperedges := C1; hypervertices := ∅ |}  <- (k +++ i)
   ) (compose_graphs_unsafe
   ( stack_graphs_aux (k -> ∅ <- k)
-                 (i -> {| hyperedges := L1; hypervertices := ∅ |} <- j)
+                 (i -> L1 <- j)
   ) (
   k +++ j -> {| hyperedges := C2; hypervertices := H.(hypervertices) |} <- H.(outputs)
   )).
@@ -1980,7 +1605,7 @@ Definition decompose_left {n m} (G : CospanHyperGraph T n m) (L : HyperGraph T) 
       (* We rebuild the let expressions used in the decompose function.
          This helps alleviate the pain. *)
       remember ({| hyperedges := C1; hypervertices := ∅ |}) as C1'.
-      remember ({| hyperedges := L1; hypervertices := ∅ |}) as L1'.
+      (* remember ({| hyperedges := L1; hypervertices := ∅ |}) as L1'. *)
       remember ({| hyperedges := C2; hypervertices := hypervertices H |}) as C2'.
       remember (vertices_hg L1) as Lv.
       (* remember (all_vertices L1') as Lv'. *)
@@ -1991,10 +1616,13 @@ Definition decompose_left {n m} (G : CospanHyperGraph T n m) (L : HyperGraph T) 
       repeat rewrite list_to_vec_app.
       repeat rewrite list_to_set_list_to_vec.
       repeat rewrite list_to_set_elements_L.
-      remember (vertices_hg L1') as Lv'.
+      remember (vertices_hg L1) as Lv'.
       rewrite (subseteq_empty_difference_L _ (Lv' ∪ C2v)),
               (subseteq_empty_difference_L _ (C1v ∪ _)).
-      + repeat rewrite union_empty_l_L.
+      + assert (hypervertices L1 = ∅).
+        { rewrite HeqL1. simpl. reflexivity. }
+        rewrite H0.
+        repeat rewrite union_empty_l_L.
         done.
       + rewrite hg_add_vertices_empty.
         apply union_subseteq_l'.
@@ -2008,7 +1636,92 @@ Definition decompose_left {n m} (G : CospanHyperGraph T n m) (L : HyperGraph T) 
           apply intersection_subseteq_r.
   Qed.
 
+  Definition DoublePushout {n m} (H : CospanHyperGraph T n m) (G : HyperGraph T) (L : list positive) : CospanHyperGraph T n m :=
+  let C1 := all_paths_idx H L in
+  let L1 := subgraph_index H L in
+  let C2 := H.(hedges).(hyperedges) ∖ (C1 ∪ L1) in
+  let C1' := vertices_hg {| hyperedges := C1; hypervertices := ∅ |} in
+  let L1' := vertices_hg L1 in
+  let C2' := vertices_hg {| hyperedges := C2; hypervertices := H.(hypervertices) |} in
+  let i := list_to_vec(elements(L1' ∩ C1')) in
+  let j := list_to_vec(elements(L1' ∩ C2')) in
+  let k := list_to_vec(elements(C1' ∩ C2')) in
+  compose_graphs_unsafe (
+  H.(inputs) -> {| hyperedges := C1; hypervertices := ∅ |}  <- (k +++ i)
+  ) (compose_graphs_unsafe
+  ( stack_graphs_aux (k -> ∅ <- k)
+                 (i -> G <- j)
+  ) (
+  k +++ j -> {| hyperedges := C2; hypervertices := H.(hypervertices) |} <- H.(outputs)
+  )).
+
+  Locate cohg_semantic_eq.
+
 End DPO.
+
+Lemma reindex_is_isomorphic {T n m} (f : positive -> positive) (finj : Inj eq eq f) (cohg : CospanHyperGraph T n m) :
+  isomorphic cohg (relabel_graph f (reindex_graph f cohg)).
+Proof.
+  rewrite isomorphic_exists.
+  exists f, f; auto.
+Qed.
+
+
+
+Lemma DPO_equiv {n m} `{TensT : TensorLike R rO rI radd rmul req A T, !EqDecision A} 
+  (Target : CospanHyperGraph T n m) 
+  (G : HyperGraph T) (L : list positive) : 
+    (forall {o p} (v0 : vec positive o) (v1 : vec positive p), 
+      (v0 -> G <- v1) ≡ₜ (v0 -> (subgraph_index Target L) <- v1)) 
+      -> Target ≡ₜ (DoublePushout Target G L).
+  Proof.
+    intros.
+    rewrite (decompose_is_graph Target L) at 1.
+    unfold decompose, DoublePushout.
+    remember (all_paths_idx Target L) as C1.
+    remember (subgraph_index Target L) as L1.
+    remember (Target.(hedges).(hyperedges) ∖ (C1 ∪ L1)) as C2.
+    remember ({| hyperedges := C1; hypervertices := ∅ |}) as C1'.
+    remember ({| hyperedges := C2; hypervertices := hypervertices Target |}) as C2'.
+    remember (vertices_hg L1) as Lv.
+    remember (vertices_hg C1') as C1v.
+    remember (vertices_hg C2') as C2v.
+    remember (list_to_vec (elements (Lv ∩ C1v))) as i.  
+    remember (list_to_vec (elements (Lv ∩ C2v))) as j.
+    remember (list_to_vec (elements (C1v ∩ C2v))) as k.
+    assert (L1 = {| hyperedges := L1; hypervertices := ∅ |}).
+    { rewrite HeqL1; now apply hg_ext. }
+    rewrite compose_graphs_unsafe_to_compose_graphs.
+    erewrite (compose_graphs_unsafe_to_compose_graphs (T:=T)).
+    rewrite (struct_isomorphic_semantic_eq).
+    Check compose_graphs_unsafe_to_compose_graphs.
+    Search (_ ≡ᵢ _ -> _ ≡ₜ _).
+    Search "cohg_semantic_eq".
+    Search "isomorphic".
+    rewrite <- (isomorphic_cohg_syntactic_eq).
+    rewrite (compose_graphs_unsafe_to_compose_graphs 
+      (inputs Target -> C1' <- k +++ i)
+      ((compose_graphs_unsafe (stack_graphs_aux (k -> ∅ <- k) (i -> L1 <- j))
+(k +++ j -> C2' <- outputs Target)))).
+    
+    (* repeat rewrite <- compose_graphs_aux_to_compose_graphs_unsafe; try done.
+    - Check reindex_graph_isomorphic.
+      (* rewrite (reindex_is_isomorphic _ _ (inputs Target -> C1' <- k +++ i)). *)
+      Search compose_graphs_aux.
+      Search reindex_graph.
+      admit.
+    - simpl.
+      rewrite vmap_id'; [done|].
+      intros.
+      now rewrite subst_by_vec_id.
+    - simpl.
+      rewrite vmap_id'; [done|].
+      intros.
+      now rewrite subst_by_vec_id. *)
+
+    (* From here typeclass resolution is failing (which will be fixed) but
+       we can proceed manually. *)
+  Admitted.
 
   Open Scope positive.
 
